library/init/data/string/basic.lean
@@ -7,29 +7,71 @@ prelude
 import init.data.list.basic
 import init.data.char.basic
 
-def string := list char
+structure string :=
+(data : list char)
+
+def list.as_string (s : list char) : string :=
+⟨s.reverse⟩
 
 namespace string
-@[pattern] def empty : string := list.nil
+def empty : string :=
+⟨list.nil⟩
 
 instance : inhabited string :=
 ⟨empty⟩
 
+def length : string → nat
+| ⟨s⟩  := s.length
+
 instance : has_sizeof string :=
-⟨list.sizeof⟩
+⟨string.length⟩
 
-@[pattern] def str : char → string → string := list.cons
+def str : string → char → string
+| ⟨s⟩ c := ⟨c::s⟩
 
-def concat (a b : string) : string :=
-list.append b a
+def append : string → string → string
+| ⟨a⟩ ⟨b⟩ := ⟨b ++ a⟩
+
+def is_empty : string → bool
+| ⟨[]⟩ := tt
+| _    := ff
 
 instance : has_append string :=
-⟨string.concat⟩
+⟨string.append⟩
+
+def to_list : string → list char
+| ⟨s⟩ := s.reverse
+
+def pop_back : string → string
+| ⟨s⟩ := ⟨s.tail⟩
+
+def popn_back : string → nat → string
+| ⟨s⟩ n := ⟨s.dropn n⟩
+
+def intercalate (s : string) (ss : list string) : string :=
+(list.intercalate s.to_list (ss.map to_list)).as_string
+
+def fold {α} (a : α) (f : α → char → α) (s : string) : α :=
+s.to_list.foldl f a
+
+def front (s : string) : char :=
+s.to_list.head
+
+def back : string → char
+| ⟨[]⟩    := default char
+| ⟨c::cs⟩ := c
+
+def backn : string → nat → string
+| ⟨s⟩ n := ⟨s.taken n⟩
+
+def join (l : list string) : string :=
+l.foldl (λ r s, r ++ s) ""
+
 end string
 
-open list
+open list string
 
-private def utf8_length_aux : nat → nat → string → nat
+private def utf8_length_aux : nat → nat → list char → nat
 | 0 r (c::s) :=
   let n := char.to_nat c in
   if                 n < 0x80 then utf8_length_aux 0 (r+1) s
@@ -42,8 +84,10 @@ private def utf8_length_aux : nat → nat → string → nat
 | (n+1) r (c::s) := utf8_length_aux n r s
 | n     r []     := r
 
-def utf8_length : string → nat
-| s := utf8_length_aux 0 0 (reverse s)
+def string.utf8_length : string → nat
+| s := utf8_length_aux 0 0 s.to_list
+
+export string (utf8_length)
 
 private def to_nat_core : list char → nat → nat
 | []      r := r
@@ -51,4 +95,7 @@ private def to_nat_core : list char → nat → nat
   to_nat_core cs (char.to_nat c - char.to_nat '0' + r*10)
 
 def string.to_nat (s : string) : nat :=
-to_nat_core s.reverse 0
+to_nat_core s.to_list 0
+
+def char.to_string (c : char) : string :=
+str empty c
