library/data/bitvec.lean
@@ -212,7 +212,7 @@ end conversion
 
 private def to_string {n : nat} : bitvec n → string
 | ⟨bs, p⟩ :=
-  "0b" ++ (bs.reverse.map (λ b, if b then '1' else '0'))
+  "0b" ++ (bs.map (λ b : bool, if b then '1' else '0')).as_string
 
 instance (n : nat) : has_to_string (bitvec n) :=
 ⟨to_string⟩
