library/init/data/list/instances.lean
@@ -54,7 +54,7 @@ instance {α : Type u} [decidable_eq α] : decidable_eq (list α) :=
 by tactic.mk_dec_eq_instance
 
 instance : decidable_eq string :=
-list.decidable_eq
+by tactic.mk_dec_eq_instance
 
 namespace list
 
