library/init/data/string/lemmas.lean
@@ -7,15 +7,15 @@ prelude
 import init.meta
 
 namespace string
-lemma empty_ne_str (c : char) (s : string) : empty ≠ str c s :=
-begin intro h, contradiction end
+lemma empty_ne_str (c : char) (s : string) : empty ≠ str s c :=
+begin cases s, unfold str empty, intro h, injection h, contradiction end
 
-lemma str_ne_empty (c : char) (s : string) : str c s ≠ empty :=
-begin intro h, contradiction end
+lemma str_ne_empty (c : char) (s : string) : str s c ≠ empty :=
+begin cases s, unfold str empty, intro h, injection h, contradiction end
 
-lemma str_ne_str_left {c₁ c₂ : char} (s₁ s₂ : string) : c₁ ≠ c₂ → str c₁ s₁ ≠ str c₂ s₂ :=
-begin intros h₁ h₂, unfold str at h₂, injection h₂, contradiction end
+lemma str_ne_str_left {c₁ c₂ : char} (s₁ s₂ : string) : c₁ ≠ c₂ → str s₁ c₁ ≠ str s₂ c₂ :=
+begin cases s₁, cases s₂, intros h₁ h₂, unfold str at h₂, injection h₂, injection h, contradiction end
 
-lemma str_ne_str_right (c₁ c₂ : char) {s₁ s₂ : string} : s₁ ≠ s₂ → str c₁ s₁ ≠ str c₂ s₂ :=
-begin intros h₁ h₂, unfold str at h₂, injection h₂, contradiction end
+lemma str_ne_str_right (c₁ c₂ : char) {s₁ s₂ : string} : s₁ ≠ s₂ → str s₁ c₁ ≠ str s₂ c₂ :=
+begin cases s₁, cases s₂, intros h₁ h₂, unfold str at h₂, injection h₂, injection h, subst data, contradiction end
 end string
