library/init/meta/interactive_base.lean
@@ -146,36 +146,36 @@ section macros
 open interaction_monad
 open interactive
 
-private meta def parse_format : string → string → parser pexpr
+private meta def parse_format : string → list char → parser pexpr
 | acc []            := pure ``(to_fmt %%(reflect acc))
 | acc ('\n'::s)     :=
-do f ← parse_format [] s,
+do f ← parse_format "" s,
    pure ``(to_fmt %%(reflect acc) ++ format.line ++ %%f)
 | acc ('{'::'{'::s) := parse_format (acc ++ "{") s
 | acc ('{'::s) :=
-do (e, s) ← with_input (lean.parser.pexpr 0) s.reverse,
-   '}'::s ← pure s.reverse | fail "'}' expected",
-   f ← parse_format [] s,
+do (e, s) ← with_input (lean.parser.pexpr 0) s.as_string,
+   '}'::s ← return s.to_list | fail "'}' expected",
+   f ← parse_format "" s,
    pure ``(to_fmt %%(reflect acc) ++ to_fmt %%e ++ %%f)
-| acc (c::s) := parse_format (acc ++ [c]) s
+| acc (c::s) := parse_format (acc ++ c.to_string) s
 
 reserve prefix `format! `:100
 @[user_notation]
 meta def format_macro (_ : parse $ tk "format!") (s : string) : parser pexpr :=
-parse_format "" s.reverse
+parse_format "" s.to_list
 
-private meta def parse_sformat : string → string → parser pexpr
+private meta def parse_sformat : string → list char → parser pexpr
 | acc []            := pure $ pexpr.of_expr (reflect acc)
 | acc ('{'::'{'::s) := parse_sformat (acc ++ "{") s
 | acc ('{'::s) :=
-do (e, s) ← with_input (lean.parser.pexpr 0) s.reverse,
-   '}'::s ← pure s.reverse | fail "'}' expected",
-   f ← parse_sformat [] s,
+do (e, s) ← with_input (lean.parser.pexpr 0) s.as_string,
+   '}'::s ← return s.to_list | fail "'}' expected",
+   f ← parse_sformat "" s,
    pure ``(to_string %%(reflect acc) ++ to_string %%e ++ %%f)
-| acc (c::s) := parse_sformat (acc ++ [c]) s
+| acc (c::s) := parse_sformat (acc ++ c.to_string) s
 
 reserve prefix `sformat! `:100
 @[user_notation]
 meta def sformat_macro (_ : parse $ tk "sformat!") (s : string) : parser pexpr :=
-parse_sformat "" s.reverse
+parse_sformat "" s.to_list
 end macros
