tests/lean/caching_user_attribute.lean
@@ -1,7 +1,7 @@
 @[user_attribute]
 meta def foo_attr : caching_user_attribute string :=
 { name     := `foo, descr := "bar",
-  mk_cache := λ ns, return $ list.join ∘ list.map (list.append "\n" ∘ to_string) $ ns,
+  mk_cache := λ ns, return $ string.join (list.map (λ n, to_string n ++ "\n") ns),
   dependencies := [] }
 
 attribute [foo] eq.refl eq.mp
