tests/lean/utf8.lean
@@ -1,9 +1,9 @@
-open list
+--open list
 
-#eval length "α₁"
-#eval length "α₁ → β₁"
-#eval length "∀ α : nat → nat, α 0 ≥ 0"
+#eval "α₁".length
+#eval "α₁ → β₁".length
+#eval "∀ α : nat → nat, α 0 ≥ 0".length
 #print "------------"
-#eval utf8_length "α₁"
-#eval utf8_length "α₁ → β₁"
-#eval utf8_length "∀ α : nat → nat, α 0 ≥ 0"
+#eval "α₁".utf8_length
+#eval "α₁ → β₁".utf8_length
+#eval "∀ α : nat → nat, α 0 ≥ 0".utf8_length
